examples/unit-tests/mac.fst
@@ -1,0 +1,103 @@
+module MacIdeal 
+open Array
+type bytes    = seq byte
+type text     = bytes
+type nbytes (n:nat) = b:bytes{length b == n}
+let macsize = 20
+let keysize = 16
+type mac_t = nbytes macsize
+type key   = nbytes keysize
+
+type key_prop : key -> text -> Type
+type pkey (p:(text -> Type)) = k:key{key_prop k == p}
+
+assume val new_key: p:(text -> Type)
+                 -> pkey p
+
+assume val hmac_sha1: key -> text -> Tot mac_t
+
+type entry = 
+  | Entry : k:key
+         -> t:text{key_prop k t}
+         -> m:mac_t
+         -> entry
+
+assume val log : ref (list entry)
+
+val mac: k:key
+      -> t:text{key_prop k t}
+      -> mac_t
+let mac k t = 
+  let m = hmac_sha1 k t in
+  log := Entry k t m :: !log;
+  m
+
+val verify: k:key
+         -> t:text 
+         -> mac_t 
+         -> b:bool{b ==> key_prop k t}
+let verify k t m = 
+  let found = List.find (function (Entry k' t' _) -> k=k' && t=t') !log in
+  is_Some found
+
+
+
+(* module Prelude *)
+(* assume val randomBytes: n:nat -> b:bytes{length b == n} *)
+(* val find: f:(x:'a -> Tot bool) *)
+(*         -> list 'a *)
+(*         -> Tot (option (x:'a{f x == true})) *)
+
+
+(* module Mac *)
+(* open Prelude *)
+(* open Array *)
+(* open ListLemmas *)
+
+(* type bytes    = seq byte *)
+(* type text     = bytes *)
+(* type nbytes (n:nat) = b:bytes{length b == n} *)
+(* let macsize = 20 *)
+(* let keysize = 16 *)
+(* type mac      = nbytes macsize *)
+(* type key = nbytes keysize *)
+
+(* (\* If you want equality on keys, while erasing the 'P index, you need *)
+(* to be careful. *)
+
+(*   (K Good b = K Bad b) decided by comparing only the b's *)
+(*   then you may conclude Good=Bad ... which is False.  *)
+
+(*   So, either:  *)
+(*     1. disable equality on types with erased components (a bit drastic) *)
+
+(*     2. allow equality after erasure if  *)
+(*           [[v1:t1]] = v1' /\ [[v2:t2]]=v2' *)
+(*         ==> (v1'=v2' ==> v1=v2) *)
+  
+
+ 
+
+(*  *\) *)
+(* (\* type key : (text => Type) => Type = *\) *)
+(* (\*   | K : 'P:(text => Type) -> bytes -> key 'P *\) *)
+
+(* (\* type f : bytes => text => Type *\) *)
+
+(* type key : (text -> Type) -> Type = *)
+(*   | K : p:(text -> Type) -> b:key -> key p *)
+
+
+(* assume val hmac_sha1: key -> text -> mac_t *)
+
+(* val gen: unit -> key 'P *)
+(* let gen () = randomBytes keysize *)
+
+(* val mac: k:key 'P -> t:text{'P t} -> mac_t *)
+(* let mac k t = hmac_sha1 k t *)
+
+(* (\* concrete *\) *)
+(* val verify: k:key 'P -> t:text -> mac_t -> b:bool{b==true ==> 'P t} *)
+(* let verify k t m = hmac_sha1 k t = m *)
+
+(* (\*********************************************************************************\) *)
